wip on P (C V) version

coq/denot/continuity.v
@@ -70,26 +70,20 @@ Import EnvNotations.
 
 (* Definitions related to continuity *)
 
-Definition monotone (F : P Value -> P Value) : Set := 
-  forall D1 D2, (D1 ⊆ D2) -> F D1 ⊆ F D2.
-
-Definition finite (X : P Value) : Prop := 
-  exists E, (X ≃ mem E) /\ E <> nil.
-
-Definition continuous (F : P Value -> P Value) : Set :=
+Definition continuous {B} (F : P Value -> P B) : Set :=
   forall X E, mem E ⊆ F X -> valid X 
          -> exists D, (mem D ⊆ X) /\ ((mem E) ⊆ F (mem D)) /\ valid_mem D.
 
-Definition monotone_env (D : Rho -> P Value) := 
-  forall ρ ρ' , ρ ⊆e ρ' -> (D ρ) ⊆ D ρ'.
-
 Definition finite_env : Rho -> Type := Env.ForallT finite.
 
-Definition continuous_In (D:Rho -> P Value) (ρ:Rho) (v:Value) : Prop :=
+Definition continuous_In {B} (D:Rho -> P B) (ρ:Rho) (v:B) : Prop :=
   v ∈ D ρ -> exists ρ' , exists (pf : finite_env ρ'),  ρ' ⊆e ρ /\ (v ∈ D ρ').
 
-Definition continuous_env (D:Rho -> P Value) (ρ:Rho) : Prop :=
-  forall v, continuous_In D ρ v.
+Definition continuous_Included {B} (D:Rho -> P B) (ρ:Rho) (X: P B) : Prop :=
+  finite X -> X ⊆ D ρ -> exists ρ' , exists (pf : finite_env ρ'),  ρ' ⊆e ρ /\ (X ⊆ D ρ').
+
+Definition continuous_env {B} (D:Rho -> P B) (ρ:Rho) : Prop :=
+  forall v, continuous_Included D ρ v.
 
 (* -------------------------------------- *)
 
@@ -107,36 +101,22 @@ Ltac gather_atoms ::=
 
 (* -- monotonicity -- *)
 
+(*
 Lemma access_monotone {ρ ρ':Rho}{x} : ρ ⊆e ρ' -> ρ ⋅ x ⊆ ρ' ⋅ x.
 Proof.
   induction 1. simpl. reflexivity.
   simpl. destruct (x == x0) eqn:E. auto.
   auto. 
-Qed.
+Qed. *)
 
 (*  forall ρ ρ', ρ ⊆e ρ' -> denot t ρ ⊆ denot t ρ'. *)
 Lemma denot_monotone {t}: 
   monotone_env (denot t).
 Proof.
   unfold monotone_env.
-  eapply tm_induction with (t := t);
-  [move=>i|move=>y|move=>t1 t2 IH1 IH2|move=> t' IH|move=>k| | | move=> t1 t2 IH1 IH2].
- all: intros ρ ρ' S.
- all: autorewrite with denot.
- all: try solve [reflexivity].
-  + eapply access_monotone; auto.
-  + eapply APPLY_mono_sub; eauto.
-  + pick fresh x.
-    repeat rewrite (denot_abs x).
-    fsetdec.
-    fsetdec.
-    eapply Λ_ext_sub.
-    intros X NE.
-    eapply IH. fsetdec.
-    eapply extend_sub_env; eauto. 
-  + eapply CONS_mono_sub; eauto.
+  intros. 
+  eapply Proper_sub_denot; auto.
 Qed.
-
 
 
 (* denot-monotone-one *)
@@ -232,20 +212,20 @@ Qed.
    set of some element in ρ x *)
 Definition initial_finite_env (ρ : Rho) (NE : valid_env ρ) : Rho.
   induction NE. exact nil.
-  destruct f as [[V _] _].
+  destruct f as [V _].
   exact (cons (x, ⌈ V ⌉) IHNE).
 Defined.
 
 Lemma initial_finite_dom : forall E NE, dom (initial_finite_env E NE) = dom E.
 Proof.
   induction NE; simpl. auto.
-  destruct f as [[v _] w].  simpl. congruence.
+  destruct f as [v w].  simpl. congruence.
 Qed. 
 
 #[export] Hint Rewrite initial_finite_dom : rewr_list.
 
-Lemma finite_singleton : forall v, finite ⌈ v ⌉.
-Proof. intros v.  exists (cons v nil).
+Lemma finite_singleton : forall {B} (v : B), finite ⌈ v ⌉.
+Proof. intros B v.  exists (cons v nil).
        repeat split; eauto. done. 
 Qed.
 
@@ -257,7 +237,7 @@ Lemma initial_fin (ρ : Rho) (NE : valid_env ρ) :
 Proof.
   induction NE.
   simpl. econstructor.
-  simpl. destruct f as [[v _] w1 ].
+  simpl. destruct f as [v w1 ].
   econstructor; eauto.
   rewrite initial_finite_dom. auto.
 Qed.
@@ -269,7 +249,7 @@ Lemma initial_fin_sub (ρ : Rho) (NE : valid_env ρ) :
   initial_finite_env ρ NE ⊆e ρ.
 Proof.
   induction NE; simpl. econstructor.
-  destruct f as [[v wpx] _].
+  destruct f as [v fx].
   econstructor. auto.
   rewrite initial_finite_dom. auto.
   intros z y. inversion y. subst. unfold In. auto.
@@ -284,30 +264,32 @@ Definition single_env (x : atom) (D : P Value) (ρ : Rho)
   update x D (initial_finite_env ρ NE).
 
   
-Lemma single_fin { v x ρ NE } : 
-  finite_env (single_env x ⌈ v ⌉ ρ NE).
+Lemma single_fin { X x ρ NE } : 
+  finite X ->
+  finite_env (single_env x X ρ NE).
 Proof.
-  induction NE; unfold finite_env; eauto.
+  induction NE; intro FIN; unfold finite_env; eauto.
   unfold single_env; econstructor.
   unfold single_env. simpl. 
-  destruct f as [[v1 I1] v2].
+  destruct f as [v1 v2].
   destruct (x == x0) eqn:EQ.
   + subst. rewrite update_eq_var. 
     econstructor.
     eapply initial_fin. simpl_env. auto. auto.
   + rewrite update_neq_var; eauto.
     econstructor; eauto.
+    eapply IHNE; eauto.
     simpl_env. auto.
 Qed.
 
 #[global] Hint Resolve single_fin : core. 
 
 
-Lemma single_sub { ρ x v } :
+Lemma single_sub { ρ x V } :
   forall (NE : valid_env ρ),
-    v ∈ ρ ⋅ x 
+    V ⊆ ρ ⋅ x 
   -> x `in` dom ρ
-  -> (single_env x ⌈ v ⌉ ρ NE) ⊆e ρ.
+  -> (single_env x V ρ NE) ⊆e ρ.
 Proof.
   intros NE.
   induction NE.
@@ -316,12 +298,11 @@ Proof.
   + (* cons case *)
     unfold single_env in *.
     simpl. simpl_env in Indom.
-    destruct f as [[w h1] h2]. simpl.
+    destruct f as [w h2]. simpl.
     simpl in vpe.
     destruct (x == x0).
     ++ subst. econstructor; eauto.
        simpl_env.  eauto.
-       intros x h. inversion h. subst. auto.
     ++ econstructor; eauto. 
        eapply IHNE; eauto. fsetdec.
        simpl_env. auto.
@@ -331,6 +312,20 @@ Qed.
 #[export] Hint Resolve single_sub : core. 
 
 
+Lemma update_access : forall {x ρ NE X},
+  x `in` dom ρ ->
+  X ≃ (single_env x X ρ NE) ⋅ x.
+Proof.
+  intros.
+  unfold single_env.
+  move: NE.
+  induction NE. fsetdec.
+  simpl. destruct f as [w h2]. simpl.
+  destruct (x == x0) eqn:EQ. subst. simpl.
+  rewrite eq_dec_refl. reflexivity.
+  simpl. rewrite EQ. eapply IHNE; auto. simpl in H. fsetdec.
+Qed.  
+
 (* v∈single[xv]x  *)
 Lemma v_single_xvx {v x ρ NE} : 
   x `in` dom ρ ->
@@ -339,7 +334,7 @@ Proof.
   unfold single_env.
   move: NE.
   induction NE; intro h. fsetdec.
-  simpl. destruct f as [[w h1] h2]. simpl.
+  simpl. destruct f as [w h2]. simpl.
   destruct (x == x0) eqn:EQ. subst. simpl.
   rewrite eq_dec_refl. econstructor; eauto.
   simpl. rewrite EQ. simpl in h. eapply IHNE; auto. fsetdec.
@@ -348,7 +343,8 @@ Qed.
 #[export] Hint Resolve v_single_xvx : core. 
 
 (* continuous-∈⇒⊆ *)
-Lemma continuous_In_sub E ρ (NE : valid_env ρ) :
+(*
+Lemma continuous_In_sub {A} (E : Rho -> (P A)) ρ (NE : valid_env ρ) :
    monotone_env E
    -> forall V, mem V ⊆ E ρ
    -> (forall v, v ∈ mem V -> continuous_In E ρ v)
@@ -380,11 +376,33 @@ Proof.
     eapply me. eapply join_sub_right; eauto. auto. 
     eapply me. eapply join_sub_left; eauto. auto.
 Qed.
-
+*)
 (* --------------------------------------- *)
 
 (* Operations are continuous *)
 
+Search Singleton.
+
+Lemma In_Included : forall {A}{x:A}{D},  x ∈ D -> ⌈ x ⌉ ⊆ D.
+Proof. 
+  intros.
+  intros y h.
+  inversion h. subst. auto.
+Qed.
+
+Lemma Included_In : forall {A}{x:A} {D},   ⌈ x ⌉ ⊆ D -> x ∈ D.
+Proof. 
+  intros.
+  apply H. eauto.
+Qed.
+
+Lemma finite_Singleton : forall {A}{x:A}, finite ⌈ x ⌉.
+Proof.
+  econstructor; eauto.
+  instantiate (1 := (x :: nil)). split; auto.
+  split; eauto using mem_singleton, singleton_mem.
+  done.
+Qed. 
 
 Lemma CONS_continuous {D E ρ}{w} :
     w ∈ (CONS (D ρ) (E ρ))
@@ -399,9 +417,9 @@ Proof.
   destruct l. try done.
   move: C => [Dv El].
   intros IHD IHE mD mE.
-  destruct (IHD v Dv) as 
+  destruct (IHD ⌈ v ⌉ finite_Singleton (In_Included Dv)) as 
       [ ρ1 [ fρ1 [ ρ1ρ VwDp1 ]]].
-  destruct (IHE (v_list l) El) as 
+  destruct (IHE ⌈ v_list l ⌉ finite_Singleton (In_Included El)) as 
       [ ρ2 [ fρ2 [ ρ2ρ VwDp2 ]]].
   have S1: same_scope ρ1 ρ. eapply Forall2_same_scope; eauto.
   have S2: same_scope ρ2 ρ. eapply Forall2_same_scope; eauto.
@@ -417,6 +435,47 @@ Proof.
 Qed.
 
 
+
+(*  BIND2 S K := exists U : P A, (RET2 U ⊆ S) /\ K U t *)
+
+Lemma BIND2_continuous {A B}{D : Rho -> M A}{K : P A -> M B}{ρ}{v} :
+  valid_env ρ ->
+  v ∈ BIND2 (D ρ) K -> 
+  continuous_env D ρ ->
+  monotone_env D  ->
+  forall E, K = (fun v => E v ρ) ->
+  (forall v, continuous_env (E v) ρ) ->
+  (forall v, monotone_env (E v)) ->
+  exists ρ', exists (pf:finite_env ρ'),
+            ρ' ⊆e ρ /\ (v ∈ BIND2 (D ρ') (fun v => E v ρ')). 
+Proof.
+  intros VE H IHD mD E -> IHE mE. 
+  move: H => [U [h1 [h2 h3]]].
+  specialize (IHE U).
+  specialize (mE U).
+  have NE : finite (RET2 U). { inversion h1. destruct H. unfold RET2. econstructor; eauto. rewrite H. 
+                               instantiate (1 := fmap pure_Comp x). split. admit. admit. }
+  edestruct (IHD _  NE h2) as 
+      [ ρ1 [ fρ1 [ ρ1ρ VwDp1 ]]].
+  edestruct (IHE ⌈ v ⌉ finite_Singleton (In_Included h3)) as 
+      [ ρ2 [ fρ2 [ ρ2ρ VwDp2 ]]].
+  have S1: same_scope ρ1 ρ. eapply Forall2_same_scope; eauto.
+  have S2: same_scope ρ2 ρ. eapply Forall2_same_scope; eauto.
+  have SS: same_scope ρ1 ρ2. { transitivity ρ; auto. symmetry; auto. }
+  exists (ρ1 ⊔e ρ2).
+  repeat split.
+  + eapply join_finite_env; eauto.
+  + eapply join_lub; eauto.
+  + unfold Ensembles.In.
+    unfold BIND2.
+    exists U. repeat split. auto. transitivity (D ρ1). auto.
+    eapply mD.
+    eapply join_sub_left; eauto.
+    eapply Included_In.
+    transitivity (E U ρ2); auto.
+    apply mE. eapply join_sub_right; eauto. 
+Admitted.
+
 Lemma APPLY_continuous {D E ρ}{w} :
   (valid_env ρ)
   -> w ∈ ((D ρ) ▩ (E ρ))
@@ -430,19 +489,11 @@ Lemma APPLY_continuous {D E ρ}{w} :
 Proof.  
   intros NE APP. inversion APP; subst. 
   all: intros IHD IHE mD mE.
-  + destruct (IHD v_wrong H) as
+  + destruct (IHD ⌈ V ↦ w ⌉ finite_Singleton (In_Included H)) as 
       [ ρ1 [ fρ1 [ ρ1ρ VwDp1 ]]].
-    exists ρ1. exists fρ1. split. auto.
-    eapply FUNWRONG; auto.
-  + destruct (IHE v_wrong H) as 
-      [ ρ1 [ fρ1 [ ρ1ρ VwDp1 ]]].
-    exists ρ1. exists fρ1. split. auto.
-    eapply ARGWRONG; auto.
-  + destruct (IHD (V ↦ w) H) as 
-      [ ρ1 [ fρ1 [ ρ1ρ VwDp1 ]]].
-    destruct 
-      (continuous_In_sub E ρ NE mE V)
-      as [ ρ2 [ fρ2 [ ρ2ρ VEp2 ]]]; eauto.
+    have NEV: finite (mem V). admit. (* {  unfold valid_mem in H1. destruct V; try done. econstructor; eauto. } *)
+    destruct (IHE (mem V) ltac:(eauto) H0) as 
+      [ ρ2 [ fρ2 [ ρ2ρ VEp2 ]]]; eauto.
     have S1: same_scope ρ1 ρ. eapply Forall2_same_scope; eauto.
     have S2: same_scope ρ2 ρ. eapply Forall2_same_scope; eauto.
     have SS: same_scope ρ1 ρ2. { transitivity ρ; auto. symmetry; auto. }
@@ -450,16 +501,15 @@ Proof.
     repeat split.
   - eapply join_finite_env; eauto.
   - eapply join_lub; eauto.
-  - have VwDp3 : V ↦ w ∈ D (ρ1 ⊔e ρ2).
-    { eapply mD. 2: eapply VwDp1. 
+  - have VwDp3 : ⌈ V ↦ w ⌉ ⊆ D (ρ1 ⊔e ρ2).
+    { transitivity (D ρ1); auto. eapply mD. 
       eapply join_sub_left. auto. }
     have VEρ3 : mem V ⊆ E (ρ1 ⊔e ρ2).
-    { intros v vV. eapply mE.
-      2: eapply VEp2; auto. 
+    { transitivity (E ρ2); auto. eapply mE.
       eapply join_sub_right.  auto. }
     eapply BETA with (V:=V); auto.
- + destruct (IHD (v_list VS)) as [ρ1 [F1 [h1 h2]]]; auto.
-   destruct (IHE (v_nat k)) as [ρ2 [F2 [h3 h4]]]; auto.
+ + destruct (IHD ⌈ v_list VS ⌉ ) as [ρ1 [F1 [h1 h2]]]; auto using In_Included, finite_Singleton.
+   destruct (IHE ⌈ v_nat k ⌉ ) as [ρ2 [F2 [h3 h4]]]; auto using In_Included, finite_Singleton.
     have S1: same_scope ρ1 ρ. eapply Forall2_same_scope; eauto.
     have S2: same_scope ρ2 ρ. eapply Forall2_same_scope; eauto.
     have SS: same_scope ρ1 ρ2. { transitivity ρ; auto. symmetry; auto. }
@@ -470,14 +520,14 @@ Proof.
   - eapply PROJ with (VS := VS) (k:=k); eauto.
     eapply mD. eapply join_sub_left; auto. auto.
     eapply mE. eapply join_sub_right; auto. auto.
- +  destruct (IHD x) as [ρ1 [F1 [h1 h2]]]; auto.
+ +  destruct (IHD ⌈ x ⌉) as [ρ1 [F1 [h1 h2]]]; auto using In_Included, finite_Singleton.
     eexists.
     eexists.
     eauto.
     split; eauto.
     eapply APPWRONG with (x:=x); auto.
- +  destruct (IHE x) as [ρ2 [F1 [h1 h2]]]; auto.
-    destruct (IHD (v_list VS)) as [ρ1 [F2 [h01 h02]]]; auto.
+ +  destruct (IHE ⌈ x ⌉) as [ρ2 [F1 [h1 h2]]]; auto using In_Included, finite_Singleton.
+    destruct (IHD ⌈ v_list VS ⌉) as [ρ1 [F2 [h01 h02]]]; auto using In_Included, finite_Singleton.
     have S1: same_scope ρ1 ρ. eapply Forall2_same_scope; eauto.
     have S2: same_scope ρ2 ρ. eapply Forall2_same_scope; eauto.
     have SS: same_scope ρ1 ρ2. { transitivity ρ; auto. symmetry; auto. }
@@ -488,7 +538,7 @@ Proof.
     - eapply PROJWRONG with (VS := VS); eauto.
     eapply mD. eapply join_sub_left; auto. auto.
     eapply mE. eapply join_sub_right; auto. auto.
-Qed.
+Admitted.
 
 
 
@@ -520,15 +570,17 @@ Proof.
   induction v.
   all: try solve [intros; cbv in H; done].
   - (* v is l ↦ v *)
-    intros [ wEVρ [NW CL] ] IH mE.
-    have VV: valid_mem l. unfold valid_mem. split; eauto.
-    destruct (IH l ltac:(eauto) v wEVρ) as
+    intros [ wEVρ NW ] IH mE.
+    have VV: valid_mem l. unfold valid_mem. eauto.
+    destruct (IH l ltac:(eauto) ⌈ c ⌉ finite_Singleton (In_Included wEVρ)) as
       [ ρ' [ fρ' [ ρ'Vρ wEρ' ]]]. 
     inversion ρ'Vρ. subst. clear ρ'Vρ.
     inversion fρ'. subst. clear fρ'.
     exists E1. exists X.
     repeat split; eauto.
-    eapply mE. 2: exact wEρ'.
+    eapply Included_In.
+    transitivity (E (x ~ a1 ++ E1)); auto.
+    eapply mE. 
     have SS: E1 ⊆e E1. eapply Reflexive_sub_env.  eapply Forall2_uniq1; eauto. 
     auto.
   - exists (initial_finite_env ρ NE).
@@ -537,6 +589,22 @@ Qed.
 
 
 (* ---------------- Denotation is continuous ----------------- *)
+
+Lemma Included_RET2 {A}{v:M A}{Y}: (v ⊆ RET2 Y) ->  exists X, (v ≃ RET2 X) /\ (X ⊆ Y).
+Proof.
+  intros.
+  cbv in H.
+  exists (fun x => Y x /\ v (ret x)).
+  repeat split.
+  - cbv. intros x vx.
+    move: (H x vx) => [b [Yb mm]].
+    exists b. repeat split; auto. inversion mm. subst. auto.
+  - cbv. intros x [b [[Yb vb] xb]]. 
+    inversion xb. subst. auto.
+  - intros y Iny.
+    destruct Iny. auto.
+Qed.
+  
 
 
 (* ⟦⟧-continuous *)
@@ -547,29 +615,47 @@ Proof.
   eapply tm_induction with (t := t);
   [move=>i|move=>x|move=>t1 t2 IH1 IH2|move=> t' IH|move=>k| | | move=> t1 t2 IH1 IH2].
   all: intros ρ NE.
-  all: intros v vIn.
-  all: autorewrite with denot in vIn.
+  all: intros m NEm mSub.
+  all: autorewrite with denot in mSub.
   all: try solve [ exists (initial_finite_env ρ NE);
     eexists; eauto] .
-  + destruct (FSetDecideAuxiliary.dec_In x (dom ρ)).
-    - exists (single_env x ⌈ v ⌉ ρ NE).
-      exists (@single_fin v x ρ NE).
+  + exfalso. destruct NEm. admit. (* eapply mSub.  eauto.  *)
+  + move: (Included_RET2 mSub) => [X [E S]].
+    destruct (FSetDecideAuxiliary.dec_In x (dom ρ)).
+    - exists (single_env x X ρ NE).
+      split.
+      have FX: finite X. admit.
+      eapply single_fin; eauto.
       split.
       ++ eapply single_sub; auto.
-      ++ eapply v_single_xvx. auto. 
+      ++ rewrite denot_var. 
+         rewrite E.
+         eapply RET2_monotone.
+
+         move: (@v_single_xvx a x ρ NE ltac:(auto)) => h.
+         
+         transitivity (RET2 (ρ ⋅ x)); auto.
+         eapply RET2_monotone.
+         intros w wIn.
+         eapply v_single_xvx. auto. 
     - exists (initial_finite_env ρ NE).
       eexists; eauto. split. eauto.
       rewrite denot_var.
+      rewrite <- ret_In_RET2.
       rewrite access_fresh. simpl_env. auto.
-      rewrite access_fresh in vIn. auto. done.
-  + edestruct (APPLY_continuous NE vIn) as [ρ' [F SS]]; eauto.
+      rewrite access_fresh in h1. auto. done.
+  + edestruct (BIND2_continuous NE vIn) as [ρ' [F [SS BB]]]; eauto.
+    instantiate (1 :=  (fun ρ v1 => BIND2 (denot t2 ρ) (fun v2 : P Value => v1 ▩ v2))). reflexivity.
     eapply denot_monotone.
-    eapply denot_monotone.
+    (* edestruct (APPLY_continuous NE vIn) as [ρ' [F SS]]; eauto. *)
+    simpl in BB.
     exists ρ'. exists F.
     rewrite denot_app. auto.
   + pick fresh x.
     rewrite (denot_abs x) in vIn. fsetdec.
-    move: (@Lambda_continuous _ _ NE v x vIn) => h.    
+    move: vIn => [v1 [h1 h2]].
+    inversion h2; subst; clear h2.
+    move: (@Lambda_continuous _ _ NE v1 x h1) => h.    
     destruct h as [ρ' [Fρ' [S vvIn]]].
     ++ intros V NEV NW.
        move: (valid_nonempty_mem _ NEV) => [w h0]. 
@@ -578,9 +664,15 @@ Proof.
     ++ exists ρ'. exists Fρ'. 
        erewrite <- Forall2_dom in Fr. 2: eapply S.
        rewrite (denot_abs x). fsetdec.
-       split; auto.
-  + edestruct (CONS_continuous vIn) as [ρ' [F SS]]; eauto.
+       repeat split; auto.
+       erewrite <- ret_In_RET2.
+       auto.
+  + edestruct (BIND2_continuous NE vIn) as [ρ' [F [SS BB]]]; eauto.
+    instantiate (1 :=  (fun ρ v1 => BIND2 (denot t2 ρ) (fun v2 : P Value => RET2 (CONS v1 v2)))). reflexivity.
     eapply denot_monotone.
+
+    edestruct (CONS_continuous vIn) as [ρ' [F SS]]; eauto.
+
     eapply denot_monotone.
     exists ρ'. exists F.
     rewrite denot_tcons. auto.
