coq/denot/definitions.v
@@ -50,30 +50,77 @@ Local Open Scope set_scope.
 
 (* Sets of Values:   P Value === Value -> Prop *)
 
+(* ----------------------------------------------------------- *)
+
+(* Computations that can fail or produce multiple results. *)
+
+Inductive Comp (v : Type) : Type := 
+  (* dynamic type error *)
+  | c_wrong : Comp v
+
+  (* multiple results *)
+  | c_multi : list v -> Comp v.
+
+#[export] Hint Constructors Comp : core.
+
+Arguments c_wrong {_}.
+Arguments c_multi {_}.
+
+Definition pure_Comp {A} (x : A) : Comp A := c_multi (x :: nil).
+
+Definition fmap_Comp {A B} (f : A -> B) (m : Comp A) : Comp B :=
+  match m with 
+  | c_wrong => c_wrong
+  | c_multi xs => c_multi (List.map f xs)
+  end.
+
+Definition append_Comp {A} (m : Comp A) (n : Comp A) : Comp A :=
+  match m with 
+  | c_wrong => c_wrong
+  | c_multi xs => match n with 
+                 | c_wrong => c_wrong
+                 | c_multi ys => c_multi (xs ++ ys)
+                 end
+  end.
+      
+Definition concat_Comp {A} (l : list (Comp A)) : Comp A :=
+  fold_right append_Comp (c_multi nil) l.
+
+Definition join_Comp {A} (m : Comp (Comp A)) : Comp A :=
+  match m with 
+  | c_wrong => c_wrong
+  | c_multi xs => concat_Comp xs
+  end.
+      
+Definition bind_Comp {A B} (m : Comp A) (k : A -> Comp B) : Comp B :=
+  join_Comp (fmap_Comp k m).
+
+#[global] Instance Monad_Comp : Monad Comp.
+split. exact @pure_Comp. exact @bind_Comp. Defined.
+
+(* ----------------------------------------------------------- *)
+
 Inductive Value : Type :=
   (* natural number *)
   | v_nat : nat -> Value
 
   (* one entry in a function's table *)
-  (* list Value is Finite set of values here *)
-  | v_map : list Value -> Value -> Value
+  | v_map : list Value -> Comp Value -> Value
 
   (* trivial function value, evaluated to a value but never applied *)
   | v_fun : Value
 
   (* list/tuple of values *)
-  | v_list : list Value -> Value
+  | v_list : list Value -> Value.
 
-  (* dynamic type error *)
-  | v_wrong : Value
-.
+(* EXAMPLE
 
-(* 
+Denotation of Identity function (\x.x):  
 
-Denotation of Identity function (\x.x):
+  any subset of 
 
- {  v_map (v_nat 1 :: nil) (v_nat 1), (2 :: nil) |-> 2, 3 |-> 3 
- } 
+ { vfun } `union` 
+ { v_map (v_nat vi :: nil) (c_multi (v_nat vi) :: nil)  | for any value vi } 
 
  *)
 
@@ -81,24 +128,25 @@ Denotation of Identity function (\x.x):
 
 Infix "↦" := v_map (at level 85, right associativity).
 
-(* A successful value is not wrong. *)
-Definition success (v : Value) : Prop :=
-  match v with 
-  | v_wrong => False
-  | _ => True
-  end.
 
-(* ------------ Valid or a denotation that "succeeds" ------------------ *)
+(* ------------ Valid values and computations ------------------ *)
+
 
 Definition valid (V : P Value) : Type :=
-  nonemptyT V * Sets.Forall success V.
+  nonemptyT V.
 
 Definition valid_mem (V : list Value) : Prop :=
-  V <> nil /\ List.Forall success V.
+  V <> nil.
+
+(* Produces at least one result *)
+
+Definition valid_Comp (C : P (Comp Value)) : Type :=
+  (nonemptyT C * not (c_wrong ∈ C) * not (c_multi nil ∈ C))%type.
+
 
 (* ------------ Semantic Operators ------------------ *)
 
-Definition WRONG : P Value := ⌈ v_wrong ⌉.
+Definition WRONG : P (Comp Value) := ⌈ c_wrong ⌉.
 
 Definition NAT : nat -> P Value :=
   fun j v => match v with 
@@ -119,11 +167,18 @@ Definition CONS : P Value -> P Value -> P Value :=
   fun V W x => 
     match x with 
     | v_list (v :: w) => (v ∈ V) /\ (v_list w ∈ W)  (* v should not be wrong *)
-(*     | v_wrong => v_wrong ∈ V *)
     | _ => False
     end.
 
-Definition Λ : (P Value -> P Value) -> P Value :=
+
+Definition CONS2 : Value -> Value -> P (Comp Value) := 
+  fun v w => match w with 
+            | v_list u => ⌈ ret (v_list (v :: u)) ⌉
+            |  _ => ⌈ c_wrong ⌉
+          end.
+
+
+Definition Λ : (P Value -> P (Comp Value)) -> P Value :=
   fun f => fun v => match v with 
           | (V ↦ w) => (w ∈ f (mem V)) /\ valid_mem V  (* CBV *)
           | v_fun => True
@@ -161,29 +216,24 @@ Inductive applicable : Value -> Prop :=
 
 #[export] Hint Constructors applicable : core.
 
-Inductive APPLY : P Value -> P Value -> (Value -> Prop) :=
-  | FUNWRONG : forall D1 D2,
-     (v_wrong ∈ D1) ->
-     APPLY D1 D2 v_wrong
-  | ARGWRONG : forall D1 D2,
-     (v_wrong ∈ D2) ->
-     APPLY D1 D2 v_wrong
+Inductive APPLY : P Value -> P Value -> (Comp Value -> Prop) :=
   | BETA : forall D1 D2 w V,
-     (V ↦ w ∈ D1) -> (mem V ⊆ D2) -> valid_mem V ->
+      (V ↦ w) ∈ D1 ->
+     (mem V ⊆ D2) -> valid_mem V ->
      APPLY D1 D2 w
   | PROJ   : forall D1 D2 w VS k, 
-     (v_list VS ∈ D1) -> (v_nat k ∈ D2) -> nth_error VS k = Some w ->
-     APPLY D1 D2 w
+     (v_list VS) ∈ D1 ->
+     (v_nat k ∈ D2) -> nth_error VS k = Some w ->
+     APPLY D1 D2 (ret w)
   | APPWRONG : forall D1 D2 x, 
-      x ∈ D1 -> success x -> not (applicable x) ->      
-      APPLY D1 D2 v_wrong
+      x ∈ D1 ->
+      not (applicable x) ->      
+      APPLY D1 D2 c_wrong
   | PROJWRONG : forall D1 D2 VS x, 
-     (v_list VS ∈ D1) -> 
-     (x ∈ D2) -> success x ->
+     (v_list VS) ∈ D1 ->
+     (x ∈ D2) -> 
      (forall k, x <> (v_nat k)) ->
-     APPLY D1 D2 v_wrong. 
-
-(* Need to add out of bounds *)
+     APPLY D1 D2 c_wrong. 
 
 Infix "▩" := APPLY (at level 90).
 
@@ -193,9 +243,9 @@ Infix "▩" := APPLY (at level 90).
 Definition ADD : P Value :=
   fun w => 
     match w with 
-    | (V ↦ v_nat k) => 
+    | (V ↦ c_multi (v_nat k :: nil)) => 
         exists i j, ((v_list (v_nat i :: v_nat j :: nil)) ∈ mem V) /\ k = i + j
-    | V ↦ v_wrong => 
+    | V ↦ c_wrong => 
         not (exists i j, v_list (v_nat i :: v_nat j :: nil) ∈ mem V) /\ valid_mem V
     | _ => False
     end.
@@ -213,11 +263,26 @@ Ltac gather_atoms ::=
   constr:(A \u B \u C \u D \u E).
 
 Module EnvNotations.
-Notation "ρ ⋅ x" := (Env.access ⌈ v_wrong ⌉ ρ x) (at level 50).
+Notation "ρ ⋅ x" := (Env.access (fun x => False) ρ x) (at level 50).
 Infix "⊔e" := (Env.map2 Union) (at level 60).
 Infix "⊆e" := (Env.Forall2 Included) (at level 50).
 End EnvNotations.
 Import EnvNotations.
+
+(* ------------------------------------------------------- *)
+
+
+Definition monotone {A}{B} (F : P A -> P B) : Set := 
+  forall D1 D2, (D1 ⊆ D2) -> F D1 ⊆ F D2.
+(* aka sub_preserving *)
+Definition sub_reflecting {A}{B} (F : P A -> P B) : Set := 
+  forall D1 D2, F D1 ⊆ F D2 -> (D1 ⊆ D2).
+
+Definition monotone_env {A} (D : Rho -> P A) := 
+  forall ρ ρ' , ρ ⊆e ρ' -> (D ρ) ⊆ D ρ'.
+
+Definition finite {B} (X : P B) : Prop := 
+  exists E, (X ≃ mem E) /\ E <> nil.
 
 (* ------------------------------------------------------- *)
 
@@ -234,150 +299,223 @@ Definition same_env : Rho -> Rho -> Prop := Env.Forall2 Same_set.
 Import LCNotations.
 Open Scope tm.
 
+(* Some properties about P and M *)
+
+#[export] Instance Monad_P : Monad P :=
+  { ret  := (fun A (x : A) => ⌈ x ⌉);
+     bind := fun A B (ca : P A) (k : A -> P B) =>
+             fun b => exists a, (a ∈ ca) /\ (b ∈ k a)
+   }.
+
+#[export] Instance Functor_P : Functor P :=
+  { fmap := fun A B (f : A -> B) (x : A -> Prop) => 
+               bind x (fun y => ret (f y)) 
+  }.
+
+#[export] Instance Applicative_P : Applicative P :=
+  { pure := @ret P _;
+     ap   := fun A B (m1 :  P (A -> B)) (m2 : P A) => 
+               bind m1 (fun x1 => 
+                            bind m2 (fun x2 => 
+                                         ret (x1 x2))) 
+  }.
+
+#[export] Instance Alternative_P : Alternative P :=
+  { empty := fun A (x:A) => False ;
+    choose := fun A (p1 p2 : P A) (y : A) => 
+                 p1 y \/ p2 y
+   }.
+
+Definition M := fun x => P (Comp x).
+
+Definition Comp_In {A} (x : A) (u : Comp A) := 
+  match u with 
+  | c_wrong => False
+  | c_multi vs => List.In x vs
+  end.
+
+Definition RET {A} : A -> M A :=
+  fun x => ⌈ ret x ⌉.
+
+Definition BIND {A B} (S : M A) (K : A -> M B) (t : Comp B) : Prop :=
+  exists (u : Comp A), exists (k : A -> Comp B), 
+    S u /\ t = bind u k /\ forall a, Comp_In a u -> K a (k a).
+
+#[export] Instance Monad_M : Monad M.
+split. exact @RET. exact @BIND. Defined.
 
 
-(* Denotation function *)
-(* `n` is is a termination metric. *)
-Fixpoint denot_n (n : nat) (a : tm) (ρ : Rho) : P Value :=
-  match n with
-  | O => fun _ => False
-  | S m => 
-     match a with 
-     | var_b _ => ⌈ v_wrong ⌉
-     | var_f x => ρ ⋅ x 
-     | app t u   => 
-         v1 <-  valid_mem V  (* CBV *)
-          | v_fun => True
-          | _ => False
-          end.
-
-(* ------------ APPLY ----------------- *)
-
-(* It is a little easier to specify this as an inductive relation 
-   than as a function. The cases don't overlap, but we don't need
-   to know that at definition time.
-*)
 
 
-(* When does APPLY diverge? (i.e. there is no w, s.t. APPLY D1 D2 w holds)
-    - D1 is empty
-    - D2 is empty
-    - D1 contains a vfun or V ↦ x, but cannot be applied to D2
-           << should this be empty or wrong??? >> 
+Definition RET2 {A} : P A -> M A := fmap pure_Comp.
 
-   When does APPLY propagate wrong?
-    - wrong in D1 or D2  (FUNWRONG / ARGWRONG) 
-    - V ↦ wrong in D1 and valid V in D2  (BETA case)
-
-   When does APPLY create a new wrong? 
-    - D1 contains a successful Value that is not a v_fun, v_map or v_list  (APPWRONG)
-    - D1 contains a v_list and D2 contains a successful Value that is not a nat (PROJWRONG)
-           
-*)
-
-Inductive applicable : Value -> Prop :=
-  | a_fun  : applicable v_fun
-  | a_list : forall VS, applicable (v_list VS)
-  | a_map  : forall V w, applicable (v_map V w).
-
-#[export] Hint Constructors applicable : core.
-
-Inductive APPLY : P Value -> P Value -> Value -> Prop :=
-  | FUNWRONG : forall D1 D2,
-     (v_wrong ∈ D1) ->
-     APPLY D1 D2 v_wrong
-  | ARGWRONG : forall D1 D2,
-     (v_wrong ∈ D2) ->
-     APPLY D1 D2 v_wrong
-  | BETA : forall D1 D2 w V,
-     (V ↦ w ∈ D1) -> (mem V ⊆ D2) -> valid_mem V ->
-     APPLY D1 D2 w
-  | PROJ   : forall D1 D2 w VS k, 
-     (v_list VS ∈ D1) -> (v_nat k ∈ D2) -> nth_error VS k = Some w ->
-     APPLY D1 D2 w
-  | APPWRONG : forall D1 D2 x, 
-      x ∈ D1 -> success x -> not (applicable x) ->      
-      APPLY D1 D2 v_wrong
-  | PROJWRONG : forall D1 D2 VS x, 
-     (v_list VS ∈ D1) -> 
-     (x ∈ D2) -> success x ->
-     (forall k, x <> (v_nat k)) ->
-     APPLY D1 D2 v_wrong. 
-
-Infix "▩" := APPLY (at level 90).
-
-
-#[export] Hint Constructors APPLY : core.
-
-Definition ADD : P Value :=
-  fun w => 
-    match w with 
-    | (V ↦ v_nat k) => 
-        exists i j, ((v_list (v_nat i :: v_nat j :: nil)) ∈ mem V) /\ k = i + j
-    | V ↦ v_wrong => 
-        not (exists i j, v_list (v_nat i :: v_nat j :: nil) ∈ mem V) /\ valid_mem V
-    | _ => False
-    end.
-
-(* ------------------------------------------------------- *)
-
-Definition Rho := Env (P Value).
-
-Ltac gather_atoms ::=
-  let A := gather_atoms_with (fun x : vars => x) in
-  let B := gather_atoms_with (fun x : var => {{ x }}) in
-  let C := gather_atoms_with (fun x => fv_tm x) in
-  let D := gather_atoms_with (fun x : list (atom * P Value) => dom x) in
-  let E := gather_atoms_with (fun x : Rho => dom x) in
-  constr:(A \u B \u C \u D \u E).
-
-Module EnvNotations.
-Notation "ρ ⋅ x" := (Env.access ⌈ v_wrong ⌉ ρ x) (at level 50).
-Infix "⊔e" := (Env.map2 Union) (at level 60).
-Infix "⊆e" := (Env.Forall2 Included) (at level 50).
-End EnvNotations.
-Import EnvNotations.
-
-(* ------------------------------------------------------- *)
-
-Definition nonempty_env : Rho -> Type := Env.ForallT nonemptyT.
-
-Definition valid_env : Rho -> Type := Env.ForallT valid. 
-
-Definition sub_env : Rho -> Rho -> Prop := Env.Forall2 Included.
-
-Definition same_env : Rho -> Rho -> Prop := Env.Forall2 Same_set.
-
-(* ------------------------------------------------------- *)
-
-Import LCNotations.
-Open Scope tm.
-
-
+(* This K wants a finite set of values from S at once 
+   so that the APPLY function can check that the domain is 
+   included in the argument. *)
+Definition BIND2 {A B} (S : P (Comp A)) (K : P A -> P (Comp B)) (t : Comp B) : Prop :=
+  exists V, finite V /\ (RET2 V ⊆ S) /\ K V t.
 
 (* Denotation function *)
 (* `n` is is a termination metric. *)
-Fixpoint denot_n (n : nat) (a : tm) (ρ : Rho) : M (P Value) :=
+Fixpoint denot_comp_n (n : nat) (a : tm) (ρ : Rho) : M Value :=
+  let fix denot_val_n (n : nat) (a : tm) (ρ : Rho) : P Value :=
   match n with
-  | O => fun _ => False
+  | O => fun x => False
   | S m => 
      match a with 
-     | var_b _ => ⌈ v_wrong ⌉
+     | var_b _ => fun x => False
+
      | var_f x => ρ ⋅ x 
-     | app t u   => 
-         denot_n m t ρ ▩ denot_n m u ρ
+
      | abs t => 
-         let x := fresh_for (dom ρ \u fv_tm t) in 
-         Λ (fun D => denot_n m (t ^ x) (x ~ D ++ ρ))
+        let x := fresh_for (dom ρ \u fv_tm t) in 
+        (Λ (fun D => (denot_comp_n m (t ^ x) (x ~ D ++ ρ))))
+
+     | tcons t u => CONS (denot_val_n m t ρ) (denot_val_n m u ρ)
+
      | lit k => NAT k
+
      | add => ADD
+
      | tnil => NIL
-     | tcons t u => CONS (denot_n m t ρ) (denot_n m u ρ)
+
+     | _ => ∅
+     end
+  end in
+  match n with
+  | O => ∅
+  | S m => 
+      match a with 
+       | app t u   => 
+           BIND2 (denot_comp_n m t ρ) (fun v1 =>
+           BIND2 (denot_comp_n m u ρ) (fun v2 =>
+           v1 ▩ v2))
+
+       | tcons t u => 
+           BIND2 (denot_comp_n m t ρ) (fun v1 =>
+           BIND2 (denot_comp_n m u ρ) (fun v2 => 
+           RET2 (CONS v1 v2 )))
+
+       | _ => RET2 (denot_val_n n a ρ)
+     end
+
+  end.
+
+Fixpoint denot_val_n (n : nat) (a : tm) (ρ : Rho) : P Value :=
+  match n with
+  | O => fun x => False
+  | S m => 
+     match a with 
+     | var_b _ => fun x => False
+
+     | var_f x => ρ ⋅ x 
+
+     | abs t => 
+        let x := fresh_for (dom ρ \u fv_tm t) in 
+        (Λ (fun D => (denot_comp_n m (t ^ x) (x ~ D ++ ρ))))
+
+     | tcons t u => CONS (denot_val_n m t ρ) (denot_val_n m u ρ)
+
+     | lit k => NAT k
+
+     | add => ADD
+
+     | tnil => NIL
+
+     | _ => ∅
      end
   end.
 
-Definition denot (a : tm) := denot_n (size_tm a) a.
+Definition denot (a : tm) := denot_comp_n (size_tm a) a.
+Definition denot_val (a : tm) := denot_val_n (size_tm a) a.
 
-Hint Opaque denot.
+#[export] Hint Opaque denot : core.
+#[export] Hint Opaque denot_val : core.
 
+
+
+Require Import Coq.Logic.PropExtensionality.
+
+Lemma ret_In_RET2 : forall {A} (U : P A) x,
+  x ∈ U <-> ret x ∈ RET2 U.
+Proof.
+  intros. 
+  unfold ret, RET2, fmap, Monad_Comp, Functor_P, bind, Monad_P, Ensembles.In.
+  split.
+  + intros Ux. exists x. split; auto.
+    cbv. econstructor.
+  + move => [a [Pa r]].
+    cbv in r. inversion r. subst. auto.
+Qed.
+
+Lemma RET2_monotone : forall {A} (U V : P A), 
+ U ⊆ V -> RET2 U ⊆ RET2 V. 
+Proof. 
+    intros A U V h x xIn.
+    destruct xIn as [ a [Ua r]].
+    inversion r. subst.
+    rewrite <- ret_In_RET2.
+    eauto.
+Qed.
+
+Lemma RET2_sub_reflecting :  forall {A} (U V : P A), 
+  RET2 U ⊆ RET2 V -> U ⊆ V.
+Proof. 
+  intros A U V h x xIn.
+  rewrite -> ret_In_RET2 in xIn.
+  specialize (h _ xIn).
+  rewrite -> ret_In_RET2.
+  auto.
+Qed.
+
+#[export] Instance Proper_Included_RET2 {A} : Proper (Included ==> Included) (@RET2 A).
+unfold Proper. intros x1 y1 E1. eapply RET2_monotone. auto. Qed.
+
+#[export] Instance Proper_Same_RET2 {A} : Proper (Same_set ==> Same_set) (@RET2 A).
+unfold Proper. intros x1 y1 E1. split. eapply RET2_monotone. rewrite E1. reflexivity.
+eapply  RET2_monotone. rewrite E1. reflexivity.
+Qed.
+
+
+
+Lemma BIND2_RET2 : forall {A B} (x : P A) (k : P A -> M B), 
+    monotone k 
+    -> finite x
+    -> BIND2 (RET2 x) k ≃ k x.
+Proof. intros. unfold BIND2, RET2.
+repeat split.
++ intros y.
+  move =>[U [h1 [h2 h3]]]. unfold M in k.
+  fold (@RET2 A) in h2.
+  eapply RET2_sub_reflecting in h2.
+  eapply (H _ _ h2). auto.
++ exists x. repeat split. eauto. reflexivity. auto.
+Qed. 
+
+
+Lemma BIND2_mono {A B} : forall (D1 D2 : M A) (K1 K2 : P A -> M B),
+  D1 ⊆ D2 -> (forall x, K1 x ⊆ K2 x) ->
+  BIND2 D1 K1 ⊆ BIND2 D2 K2.
+Proof. 
+  intros.
+  unfold BIND2.
+  move=> x [U [h1 [h2 h3]]].
+  exists U.
+  repeat split.
+  auto.
+  transitivity D1; auto.
+  specialize (H0 U x).
+  eapply H0. auto.
+Qed.
+
+#[export] Instance Proper_Included_BIND2 {A B} : Proper (Included ==> Logic.eq ==> Included) (@BIND2 A B).
+intros x1 y1 E1 x2 y2 ->. 
+eapply BIND2_mono; eauto. reflexivity.
+Qed. 
+
+#[export] Instance Proper_Same_BIND2 {A B} : Proper (Same_set ==> Logic.eq ==> Same_set) (@BIND2 A B).
+unfold Proper. intros x1 y1 E1 x2 y2 ->. split. eapply BIND2_mono. rewrite E1. reflexivity. reflexivity.
+eapply  BIND2_mono. rewrite E1. reflexivity. reflexivity.
+Qed.
+  
 
