coq/denot/valid_theory.v
@@ -26,34 +26,22 @@ Ltac forall_success :=
 
 Lemma valid_mem_valid {V} : valid_mem V -> valid (mem V).
 Proof.
-  intros [V1 V2].
+  intros V1.
   destruct V; simpl in *. done.
-  split. exists v. auto. eauto.
+  exists v. auto. 
 Qed.
 
 
 (* valid sets are inhabited *)
-Definition valid_is_nonempty V : valid V -> nonemptyT V := fst.
+Definition valid_is_nonempty V : valid V -> nonemptyT V := id.
 
 Lemma valid_nonempty_mem : forall V, 
       valid_mem V -> nonemptyT (mem V).
 Proof. intros. eapply valid_is_nonempty.
        eapply valid_mem_valid; auto. Qed.
 
-(* And do not contain wrong *)
-Lemma valid_not_wrong {X} : valid X -> not (v_wrong ∈ X).
-Proof. intros [x h1]. intro h. 
-       specialize (h1 _ h). simpl in h1. done. Qed.
-
 Lemma valid_mem_nonnil {V} : valid_mem V -> V <> nil.
-Proof. intros [h _]; auto. Qed.
-
-Lemma valid_mem_not_wrong {V} : valid_mem V -> not (List.In v_wrong V).
-Proof. intros [h j]; auto. 
-       rewrite List.Forall_forall in j.
-       intro h1.
-       specialize (j _ h1). simpl in j. done.
-Qed.
+Proof. intros h; auto. Qed.
 
 (* A finite, inhabited subset of a valid set is valid *)
 Lemma valid_sub_valid_mem {D a} :
@@ -62,29 +50,20 @@ Proof.
   intros NE [V1 V2] S.
   inversion V1.
   induction D. try done. 
-  split; auto.
-  destruct D.
-  econstructor; eauto. specialize (S a0 ltac:(eauto)). 
-  eapply V2; eauto.
-  econstructor; eauto. specialize (S a0 ltac:(eauto)). 
-  eapply V2; eauto. 
-  eapply IHD. intro h. done. intros y yIn. eapply S.
-  eauto.
+  auto. done.
+  auto. auto.
 Qed.
 
 
-#[export] Hint Immediate valid_is_nonempty valid_nonempty_mem valid_not_wrong valid_mem_valid valid_mem_nonnil valid_mem_not_wrong valid_sub_valid_mem : core.
+#[export] Hint Immediate valid_is_nonempty valid_nonempty_mem valid_mem_valid valid_mem_nonnil valid_sub_valid_mem : core.
 
 Lemma valid_join : forall v1 v2, 
     valid v1 -> 
     valid v2 ->
     valid (v1 ∪ v2).
 Proof.
-  intros v1 v2 [[x1 I1] h1] [[x2 I2] h2].
-  split. 
+  intros v1 v2 [x1 h1] [x2 h2].
   exists x1. eapply Union_introl; eauto.
-  intros x xIn. inversion xIn. subst. eapply h1; eauto.
-  eapply h2;eauto.
 Qed.
 
 
@@ -94,54 +73,44 @@ Qed.
 Lemma valid_NIL : valid NIL.
 Proof.
   unfold NIL, valid.
-  split. econstructor; eauto.
-  forall_success. inversion H0.
+  econstructor; eauto.
 Qed.
 
 Lemma valid_CONS {x y z} : valid x -> valid y -> v_list z ∈ y -> valid (CONS x y).
 Proof.
-  intros [[vx h1] nx] [[vl h2] nl] In. unfold CONS.
-  split.
+  intros [vx nx] [vl nl] In. unfold CONS.
   - exists (v_list (vx :: z)). cbv. eauto.
-  - forall_success. 
 Qed. 
 
 Lemma valid_NAT : forall k, valid (NAT k).
 Proof.
-  intros k. unfold NAT, valid. split.
+  intros k. unfold NAT, valid. 
   exists (v_nat k); eauto. cbn. auto.
-  forall_success.
 Qed.
 
 Lemma valid_ADD : valid ADD.
 Proof. 
   unfold ADD, valid.
-  split.
-  exists ( (v_list (v_nat 0 :: v_nat 0 :: nil) :: nil) ↦ v_nat 0). 
-  cbn.
+  exists ( (v_list (v_nat 0 :: v_nat 0 :: nil) :: nil) ↦ pure_Comp (v_nat 0)). 
   exists 0. exists 0. split.  auto. auto.
-  forall_success.
 Qed.
 
 Lemma valid_Λ : forall F, valid (Λ F).
 Proof. 
   intros F. 
-  split. cbv.
+  cbv.
   exists v_fun. auto. 
-  forall_success.
 Qed.
 
  
 Lemma valid_LIST : forall D, List.ForallT valid D -> valid (LIST D).
 induction 1. 
-split; auto.
-exists (v_list nil); done. forall_success.
-destruct IHX as [[xs nin] h].
-destruct p as [[y niny] hy]. 
+auto.
+exists (v_list nil); done. 
+destruct IHX as [xs h].
+destruct p as [y hy]. 
 destruct xs; try done.
-split. 
 exists (v_list (y :: l0)). econstructor; eauto.
-forall_success.
 Qed.
 
 (* Valid environments *)
