coq/denot/denot.v
@@ -1,27 +1,15 @@
 (* 
 
 This module provides rewriting rules for the denotation function, so that users need never look 
-at denot_n. These can be accessed by the "denot" Hint database.
+at the fuel-based definition. These can be accessed by the "denot" Hint database for 
+all syntactic forms except for abs.
 
 Rewriting abstractions is not automatic because the new variable name must be provided.
   
 Lemma denot_abs : forall x t ρ,
-   x `notin` dom ρ \u fv_tm t ->
-   denot (abs t) ρ = 
-     Λ (fun D => denot (t ^ x) (x ~ D ++ ρ)).
-
-It also shows the weakening and substitution properties for denot.
-   
-Lemma weaken_denot : forall t ρ2 ρ,
-   fv_tm t [<=] dom ρ2 ->
-   uniq (ρ ++ ρ2) ->
-   denot t ρ2 = denot t (ρ ++ ρ2). 
-
-Lemma subst_denot1 :
-  forall (t : tm) (x : atom) (u : tm) (ρ : Env (P Value)),
-    scoped t (x ~ denot u ρ ++ ρ) ->
-    scoped u ρ ->
-    denot t (x ~ denot u ρ ++ ρ) = denot (t [x ~> u]) ρ.
+    x `notin` dom ρ \u fv_tm t ->
+    denot (abs t) ρ = 
+      RET2 (Λ (fun D => denot (t ^ x) (x ~ D ++ ρ))).
 
  *)
 
@@ -56,59 +44,129 @@ Ltac gather_atoms ::=
   constr:(A \u B \u C \u D).
 
 
-Lemma size_is_enough : forall n a, n >= size_tm a -> forall ρ, denot_n n a ρ = denot_n (size_tm a) a ρ.
+Lemma size_is_enough_mutual : 
+  forall n a, n >=  (size_tm a) -> 
+         (forall ρ, denot_comp_n n a ρ = denot_comp_n (size_tm a) a ρ) /\
+         (forall ρ, denot_val_n n a ρ = denot_val_n (size_tm a) a ρ).
 Proof.
   intros n.
   induction (lt_wf n) as [n _ IH].
-  intros a h ρ; destruct a; simpl in *.
+
+  intros a h; split; intros ρ; destruct a; simpl in *.
+
   all: try destruct n; simpl; auto; try lia.
+
   all: f_equal.
-  all: try rewrite IH; try lia; auto;
-    try rewrite IH; try lia; auto.
-  - extensionality D.
-    remember (fresh_for (dom ρ \u fv_tm a)) as x.
-    rewrite IH. lia.
+  all: try extensionality b.
+  all: try (f_equal; extensionality a0).
+  - remember (fresh_for (dom ρ \u fv_tm a)) as x.
+    destruct (IH n ltac:(auto) (a ^ x)) as [IHC IHV].
     autorewrite with lngen. lia.
+    rewrite IHC. 
     autorewrite with lngen. auto.
+  - edestruct (IH n ltac:(lia) a1 ltac:(lia)) as [IHC1 IHV1]. 
+    edestruct (IH (size_tm a1 + size_tm a2) ltac:(lia) a1 ltac:(lia)) as [IHC2 IHV2]. 
+    rewrite IHC1. rewrite IHC2. auto. 
+  - edestruct (IH n ltac:(lia) a2 ltac:(lia)) as [IHC1 IHV1]. 
+    edestruct (IH (size_tm a1 + size_tm a2) ltac:(lia) a2 ltac:(lia)) as [IHC2 IHV2]. 
+    rewrite IHC1. rewrite IHC2. auto.      
+  - edestruct (IH n ltac:(lia) a1 ltac:(lia)) as [IHC1 IHV1]. 
+    edestruct (IH (size_tm a1 + size_tm a2) ltac:(lia) a1 ltac:(lia)) as [IHC2 IHV2]. 
+    rewrite IHC1. rewrite IHC2. auto. 
+  - edestruct (IH n ltac:(lia) a2 ltac:(lia)) as [IHC1 IHV1]. 
+    edestruct (IH (size_tm a1 + size_tm a2) ltac:(lia) a2 ltac:(lia)) as [IHC2 IHV2]. 
+    rewrite IHC1. rewrite IHC2. auto.      
+  - remember (fresh_for (dom ρ \u fv_tm a)) as x.
+    destruct (IH n ltac:(auto) (a ^ x)) as [IHC IHV].
+    autorewrite with lngen. lia.
+    rewrite IHC. 
+    autorewrite with lngen. auto.
+  - edestruct (IH n ltac:(lia) a1 ltac:(lia)) as [IHC1 IHV1]. 
+    edestruct (IH (size_tm a1 + size_tm a2) ltac:(lia) a1 ltac:(lia)) as [IHC2 IHV2]. 
+    rewrite IHV1. rewrite IHV2. auto. 
+  - edestruct (IH n ltac:(lia) a2 ltac:(lia)) as [IHC1 IHV1]. 
+    edestruct (IH (size_tm a1 + size_tm a2) ltac:(lia) a2 ltac:(lia)) as [IHC2 IHV2]. 
+    rewrite IHV1. rewrite IHV2. auto. 
 Qed.
 
-Hint Transparent denot.
-
-Lemma denot_var_b : forall x ρ, denot (var_b x) ρ = ⌈ v_wrong ⌉.
+Lemma size_is_enough : 
+  forall n a, n >=  (size_tm a) -> 
+         (forall ρ, denot_comp_n n a ρ = denot_comp_n (size_tm a) a ρ).
 Proof.
-  intros x ρ. reflexivity.
-Qed.
+  intros.
+  eapply size_is_enough_mutual. auto.
+Qed.         
 
-Lemma denot_var : forall x ρ, denot (var_f x) ρ = ρ ⋅ x.
+Lemma size_is_enough_val : 
+  forall n a, n >=  (size_tm a) -> 
+         (forall ρ, denot_val_n n a ρ = denot_val_n (size_tm a) a ρ).
+Proof.
+  intros.
+  eapply size_is_enough_mutual. auto.
+Qed.         
+
+
+Local Hint Transparent denot.
+Local Hint Transparent denot_val.
+
+
+Lemma denot_var_b : forall x ρ, denot (var_b x) ρ = fun x => False.
+Proof.
+  intros x ρ.
+  cbv. 
+  extensionality b.
+  f_equal.
+Admitted.
+
+
+Lemma denot_val_var : forall x ρ, denot_val (var_f x) ρ = ρ ⋅ x.
 Proof.
   intros. reflexivity.
 Qed.
 
+Lemma denot_var : forall x ρ, denot (var_f x) ρ = RET2 (ρ ⋅ x).
+Proof.
+  intros. reflexivity.
+Qed.
+
+
+
+
 Lemma denot_app : forall t u ρ, 
     denot (app t u) ρ = 
-      (denot t ρ ▩ denot u ρ).
+      BIND2 (denot t ρ) (fun v1 =>
+      BIND2 (denot u ρ) (fun v2 => 
+      v1 ▩ v2)).
 Proof. 
   intros.
   unfold denot. simpl.
+  f_equal.
   rewrite size_is_enough. lia. auto.
+  extensionality v1.
+  f_equal.
   rewrite size_is_enough. lia. auto.
 Qed.
 
-Lemma denot_lit : forall k ρ,  denot (lit k) ρ = NAT k.
+Lemma denot_lit : forall k ρ,  denot (lit k) ρ = RET2 (NAT k).
 Proof. intros. reflexivity. Qed. 
 
-Lemma denot_add : forall ρ,  denot add ρ = ADD.
+Lemma denot_add : forall ρ,  denot add ρ = RET2 ADD.
 Proof. intros. reflexivity. Qed. 
 
-Lemma denot_tnil : forall ρ,  denot tnil ρ = NIL.
+Lemma denot_tnil : forall ρ,  denot tnil ρ = RET2 NIL.
 Proof.  intros. reflexivity. Qed. 
 
 Lemma denot_tcons : forall t u ρ, 
-    denot (tcons t u) ρ = CONS (denot t ρ) (denot u ρ).
+    denot (tcons t u) ρ =
+      BIND2 (denot t ρ) (fun v1 =>
+      BIND2 (denot u ρ) (fun v2 =>
+      RET2 (CONS v1 v2))).
 Proof. 
   intros.
   unfold denot. simpl.
+  f_equal.
   rewrite size_is_enough. lia. auto.
+  extensionality v1. f_equal.
   rewrite size_is_enough. lia. auto.
 Qed.
 
@@ -125,15 +183,15 @@ Ltac name_binder x0 Frx0 :=
          simpl_env in Frx0
     end.    
 
-Definition access_app_P := @access_app (P Value) ⌈ v_wrong ⌉.
+Definition access_app_P := @access_app (P Value) (fun x => False).
 
 (* Renaming property for denotations. *)
 
 Lemma rename_denot_n : forall n t y w ρ1 ρ2 D, 
   w `notin` dom ρ1 -> 
   y `notin` dom ρ1 \u fv_tm t -> 
-  denot_n n t (ρ1 ++ w ~ D ++ ρ2) = 
-  denot_n n (t [w ~> var_f y]) (ρ1 ++ y ~ D ++ ρ2).
+  denot_comp_n n t (ρ1 ++ w ~ D ++ ρ2) = 
+  denot_comp_n n (t [w ~> var_f y]) (ρ1 ++ y ~ D ++ ρ2).
 Proof. 
   induction n;
   intros t y w ρ1 ρ2 D Frw Fry; simpl. auto.
@@ -174,10 +232,12 @@ Proof.
       fsetdec.
       auto.
     } 
+    f_equal. 
+    extensionality D1.
     rewrite <- cons_app_assoc.
 
-    replace (((x0, D0) :: ρ1) ++ (w, D) :: ρ2) with
-      (nil ++ (x0 ~ D0) ++ (ρ1 ++ (w ~ D) ++ ρ2)). 2: { simpl_env; auto. }
+    replace (((x0, D1) :: ρ1) ++ (w, D) :: ρ2) with
+      (nil ++ (x0 ~ D1) ++ (ρ1 ++ (w ~ D) ++ ρ2)). 2: { simpl_env; auto. }
     rewrite <- IHn; simpl_env; auto.
     2: { autorewrite with lngen. 
          clear Fry0 Frw Fry.
@@ -185,8 +245,8 @@ Proof.
          fsetdec.
     }
 
-    replace ((y0 ~ D0) ++ ρ1 ++ (y ~ D) ++ ρ2) with
-      (nil ++ (y0 ~ D0) ++ (ρ1 ++ (y ~ D) ++ ρ2)). 2: { simpl_env; auto. }
+    replace ((y0 ~ D1) ++ ρ1 ++ (y ~ D) ++ ρ2) with
+      (nil ++ (y0 ~ D1) ++ (ρ1 ++ (y ~ D) ++ ρ2)). 2: { simpl_env; auto. }
 
     rewrite <- IHn; simpl_env; auto.
     2: { rewrite fv_tm_subst_tm_upper.            
@@ -197,7 +257,7 @@ Proof.
          fsetdec.
     }
     
-    repeat rewrite <- (app_assoc _ (z ~ D0)).
+    repeat rewrite <- (app_assoc _ (z ~ D1)).
     eapply IHn.
     simpl_env. { clear Fry0 Fry Frx0. fsetdec. }
     rewrite fv_tm_open_tm_wrt_tm_upper.
@@ -209,10 +269,13 @@ Proof.
   + simpl_env.
     f_equal.
     apply IHn; simpl_env; auto.
+    extensionality v1.
+    f_equal.
     apply IHn; simpl_env; auto.
   + simpl_env.
     f_equal.
     apply IHn; simpl_env; auto.
+    extensionality v1. f_equal.
     apply IHn; simpl_env; auto. 
 Qed.
 
@@ -220,8 +283,8 @@ Qed.
 Lemma rename_open_denot : forall w y n t  ρ D, 
   w `notin` fv_tm t -> 
   y `notin` fv_tm t -> 
-  denot_n n (t ^ w) (w ~ D ++ ρ) = 
-  denot_n n (t ^ y) (y ~ D ++ ρ).
+  denot_comp_n n (t ^ w) (w ~ D ++ ρ) = 
+  denot_comp_n n (t ^ y) (y ~ D ++ ρ).
 Proof. 
   intros.
   pick fresh z.
@@ -238,12 +301,12 @@ Qed.
 Lemma denot_abs : forall x t ρ,
     x `notin` dom ρ \u fv_tm t ->
     denot (abs t) ρ = 
-      Λ (fun D => denot (t ^ x) (x ~ D ++ ρ)).
+      RET2 (Λ (fun D => denot (t ^ x) (x ~ D ++ ρ))).
 Proof.
   intros.
   unfold denot. simpl.
   rewrite size_tm_open_tm_wrt_tm_var.
-  f_equal.
+  f_equal. f_equal.
   extensionality D.
   name_binder x0 Frx0.
   simpl_env. 
@@ -257,133 +320,5 @@ Create HintDb denot.
   denot_add denot_tnil denot_tcons : denot.
 (* no hint for abs, must pick fresh first *)
 
-Lemma weaken_denot1 : forall t ρ ρ1 ρ2, 
-    fv_tm t [<=] dom (ρ1 ++ ρ2) ->
-    uniq (ρ1 ++ ρ ++ ρ2) ->
-    denot t (ρ1 ++ ρ2) = denot t (ρ1 ++ ρ ++ ρ2). 
-Proof.
-  intro t.
-  eapply tm_induction with (t := t).
-  1: move=>i. 
-  2: move=>x.
-  3: move=>t1 t2 IH1 IH2. 
-  4: move=> u IH.
-  8: move=> t1 t2 IH1 IH2.
-  all: intros ρ ρ1 ρ2 FV U.
-  all: simpl_env in FV; simpl in FV. 
-  all: autorewrite with denot.
-  all: try solve [reflexivity].
-  + (* var *) 
-    destruct_uniq.
-    move: (access_app_P ρ1 x) => [A1|A2].
-    rewrite A1. rewrite A1. auto.
-    move: (A2 ρ2) => [A21 A22].
-    rewrite A22.
-    move: (A2 (ρ ++ ρ2)) => [A31 A32].
-    rewrite A32.
-    rewrite access_app_fresh; auto.
-    intro h.
-    solve_uniq.
-  + (* app *)
-    f_equal.
-    eapply IH1; simpl_env; eauto.
-    fsetdec.
-    eapply IH2; simpl_env; eauto.
-    fsetdec.
-  + pick fresh x.
-    repeat rewrite (denot_abs x).
-    simpl_env; fsetdec.
-    simpl_env; fsetdec.
-    f_equal.
-    extensionality D.
-    rewrite <- app_assoc.
-    erewrite IH; simpl_env; eauto.
-    rewrite fv_tm_open_tm_wrt_tm_upper; simpl; eauto.
-    fsetdec.
-  + f_equal.
-    eapply IH1; simpl_env; eauto.
-    fsetdec.
-    eapply IH2; simpl_env; eauto.
-    fsetdec.
-Qed.
 
-Lemma weaken_denot : forall t ρ2 ρ,
-   fv_tm t [<=] dom ρ2 ->
-   uniq (ρ ++ ρ2) ->
-   denot t ρ2 = denot t (ρ ++ ρ2). 
-Proof.
-  intros.
-  unfold denot.
-  eapply weaken_denot1 with (ρ1 := nil); simpl; auto.
-Qed.
 
-(* Scoping predicates *)
-
-Lemma subst_denot : forall t x u ρ1 ρ2, 
-    scoped t (ρ1 ++ x ~ (denot u ρ2) ++ ρ2) ->
-    scoped u ρ2 ->
-    denot t (ρ1 ++ x ~ (denot u ρ2) ++ ρ2) =
-    denot (t [x ~> u]) (ρ1 ++ ρ2).
-Proof.
-  intro t.
-  eapply tm_induction with (t := t);
-  [move=>i|move=>y|move=>t1 t2 IH1 IH2|move=> t' IH|move=>k| | | move=> t1 t2 IH1 IH2].
-  all: intros x u ρ1 ρ2 ST SU.
-  all: simpl. 
-  all: simpl_env. 
-  all: autorewrite with denot.
-  all: try solve [reflexivity].
-  + destruct (y == x) eqn:EQ. subst.
-    ++ have NI: x `notin` dom ρ1.
-       { inversion ST. destruct_uniq. auto. }
-       have D2: fv_tm u [<=] dom ρ2. 
-       { inversion SU. auto. }
-       have U2: uniq (ρ1 ++ ρ2). 
-       { inversion ST. solve_uniq. }
-       rewrite access_app_fresh; auto.       
-       rewrite access_eq_var.
-       apply weaken_denot; eauto.
-    ++ repeat rewrite denot_var.
-       destruct (access_app_P ρ1 y) as [h1 | h2].
-       repeat rewrite h1. auto.
-       move: (h2 ρ2) => [N1 ->]. 
-       move: (h2 (x ~ denot u ρ2 ++ ρ2)) => [N3 ->].
-       rewrite access_neq_var; auto.
-  + move: (scoped_app_inv1 _ _ _ _ ST) => S1.
-    move: (scoped_app_inv2 _ _ _ _ ST) => S2.
-    f_equal.
-    eapply IH1; eauto.
-    eapply IH2; eauto.
-  + have LCU: lc_tm u. inversion SU. auto.
-    pick fresh z.
-    specialize (IH z ltac:(auto) x u).
-    simpl. simpl_env.
-    repeat rewrite (denot_abs z).
-    simpl_env. fsetdec.
-    simpl_env. rewrite fv_tm_subst_tm_upper. fsetdec. 
-    f_equal.
-    extensionality D.
-    have FZ: z `notin` (dom (ρ1 ++ x ~ denot u ρ2 ++ ρ2) \u fv_tm t').
-    simpl_env. fsetdec.
-    move: (scoped_abs_inv _ z t' D _ FZ ST) => h.
-    rewrite <- app_assoc.
-    rewrite IH; auto.
-    rewrite subst_tm_open_tm_wrt_tm. eauto.
-    rewrite subst_neq_var. auto.
-    reflexivity.
-  + move: (scoped_tcons_inv1 _ _ _ _ ST) => S1.
-    move: (scoped_tcons_inv2 _ _ _ _ ST) => S2.
-    f_equal.
-    eapply IH1; eauto.
-    eapply IH2; eauto.
-Qed.
-
-Lemma subst_denot1 :
-  forall (t : tm) (x : atom) (u : tm) (ρ : Env (P Value)),
-    scoped t (x ~ denot u ρ ++ ρ) 
-    -> scoped u ρ 
-    -> denot t (x ~ denot u ρ ++ ρ) = denot (t [x ~> u]) ρ.
-Proof.
-  intros. 
-  eapply subst_denot with (ρ1 := nil); auto. 
-Qed.
